save wtf

example/Bellman_Ford.thy
@@ -1,6 +1,6 @@
 theory Bellman_Ford
-  imports "../DP_Lifting" "../DP_CRelVS" "../DP_Proof" "../scratch/Scratch_relator_mono"
-begin
+  imports "../DP_Lifting" "../DP_CRelVS" "../DP_Proof"
+begin                                        
   
 consts n :: nat
 consts W :: "nat \<Rightarrow> nat \<Rightarrow> int"
@@ -26,13 +26,6 @@ thm bf.simps
 thm bf.induct
 term 0 (**)
   
-lemma map\<^sub>T_return_return_cong[fundef_cong]:
-  fixes f g xs
-  assumes "\<And>x. x\<in>set xs \<Longrightarrow> f x = g x"
-  shows "map\<^sub>T . \<langle>f\<rangle> . \<langle>xs\<rangle> = map\<^sub>T . \<langle>g\<rangle> . \<langle>xs\<rangle>"
-  sorry
-term 0 (**)
-  
 fun bf\<^sub>T :: "nat\<times>nat \<Rightarrow>\<^sub>T int" where
   "bf\<^sub>T$ (0, j) =CHECKMEM= \<langle>W 0 j\<rangle>"
 | "bf\<^sub>T$ (Suc k, j) =CHECKMEM=
@@ -51,108 +44,426 @@ context
   includes lifting_syntax
 begin
 
-abbreviation K :: "'a \<Rightarrow> 'a \<Rightarrow> 'a \<Rightarrow> bool" where
-  "K x \<equiv> eq_onp (op = x)"
-term 0 (**)
-
 lemma bf_induct:
   "\<lbrakk>\<And>j. P (0, j);
-    \<And>k j. \<lbrakk>\<And>x. x \<in> set [0..<n] \<Longrightarrow> P (k, x);
+    \<And>k j. \<lbrakk>\<And>x. P (k, x);
            P (k, j)
            \<rbrakk> \<Longrightarrow> P (Suc k, j)
    \<rbrakk> \<Longrightarrow> P (x::nat\<times>nat)"
   by (fact bf\<^sub>T.induct)
+term 0 (**)
+term "pred_prod (op = (0::nat)) (op = (j::nat))"
+term "top::bool\<Rightarrow>bool"
+term map_fun
+term pred_fun
+lemma bf_induct':
+  "\<lbrakk>\<And>j. pred_fun (pred_prod (op = 0) (op = j)) id P;
+    \<And>k j. \<lbrakk>pred_fun (pred_prod (op = k) top) id P;
+           pred_fun (pred_prod (op = k) (op = j)) id P\<rbrakk> \<Longrightarrow> P (Suc k, j)
+   \<rbrakk> \<Longrightarrow> P (x::nat\<times>nat)"
+  subgoal premises IH
+    apply (rule bf_induct)
+    subgoal premises prems for j
+      apply (rule IH(1)[of j, unfolded pred_fun_def id_def, THEN spec, THEN mp])
+      apply (rule pred_prod.intros)
+       apply (rule refl)
+      apply (rule refl)
+      done
+    subgoal premises prems for k j
+      apply (rule IH(2)[of k j])
+      subgoal
+        unfolding pred_fun_def id_def
+        apply (rule allI, rule impI)
+        apply (erule pred_prod.induct)
+        apply (clarify)
+        apply (rule prems(1))
+        done
+      subgoal
+        unfolding pred_fun_def id_def
+        apply (rule allI, rule impI)
+        apply (erule pred_prod.induct)
+        apply clarify
+        apply (rule prems(2))
+        done
+      done
+    done
+  done
+    
+    
+term 0 (**)
 
 lemma bf_inductS:
   "\<lbrakk>\<And>j. bf.crel_vs op = (bf (0, j)) (bf\<^sub>T (0, j));
-    \<And>k j. \<lbrakk>\<And>x. x \<in> set [0..<n] \<Longrightarrow> bf.crel_vs op = (bf (k, x)) (bf\<^sub>T (k, x));
+    \<And>k j. \<lbrakk>\<And>x. bf.crel_vs op = (bf (k, x)) (bf\<^sub>T (k, x));
            bf.crel_vs op = (bf (k, j)) (bf\<^sub>T (k, j))
            \<rbrakk> \<Longrightarrow> bf.crel_vs op = (bf (Suc k, j)) (bf\<^sub>T (Suc k, j))
    \<rbrakk> \<Longrightarrow> bf.crel_vs op = (bf (x::nat\<times>nat)) (bf\<^sub>T x)"
   by (fact bf_induct)
 
-
+definition "K x \<equiv> eq_onp (op = x)"
+lemma K_self: "K x x x"
+  unfolding K_def eq_onp_def by auto
+    
+ML \<open>
+fun debug_tac th = let val _ = @{print} th in all_tac th end;
+SOLVE;
+\<close>
+  
 lemma bf_inductS':
-  "\<lbrakk>\<And>j. bf.crel_vs op = (bf (0, j)) (bf\<^sub>T (0, j));
-    \<And>k j. \<lbrakk>(rel_prod (K k) (eq_onp (\<lambda>x. x\<in>set [0..<n])) ===> bf.crel_vs op =) bf bf\<^sub>T;
+  "\<And>param.
+  \<lbrakk>\<And>j. K j j j \<Longrightarrow> bf.crel_vs op = (bf (0, j)) (bf\<^sub>T (0, j));
+    \<And>k j. \<lbrakk>K k k k; K j j j;
+           (rel_prod (K k) (op =) ===> bf.crel_vs op =) bf bf\<^sub>T;
            (rel_prod (K k) (K j) ===> bf.crel_vs op =) bf bf\<^sub>T
            \<rbrakk> \<Longrightarrow> bf.crel_vs op = (bf (Suc k, j)) (bf\<^sub>T (Suc k, j))
-   \<rbrakk> \<Longrightarrow> bf.crel_vs op = (bf (x::nat\<times>nat)) (bf\<^sub>T x)"
-  unfolding eq_onp_def rel_prod.simps using bf_inductS by blast
-term 0 (**)
-thm eq_onp_to_eq
-  
-notation bf.rel_fun_lifted (infixr "===>\<^sub>T" 55)
-  
-ML  \<open>
-fun eq_tac ctxt =
-  TRY o REPEAT_ALL_NEW (resolve_tac ctxt @{thms relator_eq_raw})
-  THEN_ALL_NEW resolve_tac ctxt @{thms is_equality_eq}
-fun tac0 ctx = REPEAT_ALL_NEW (resolve_tac ctx @{thms transfer_raw});
-fun tac1 ctx = DETERM o eq_tac ctx;
-fun transfer_step_tac ctx = tac0 ctx THEN_ALL_NEW tac1 ctx;
+   \<rbrakk> \<Longrightarrow> (\<lambda>param. bf.crel_vs op = (bf param) (bf\<^sub>T param)) (param::nat\<times>nat)"
+  apply (tactic \<open>
+    HEADGOAL (Subgoal.FOCUS (fn {context=ctxt1, prems=IH, ...} => HEADGOAL (
+      resolve_tac ctxt1 @{thms bf\<^sub>T.induct}
+      THEN_ALL_NEW (fn i => Subgoal.FOCUS (fn {context=ctxt2, prems, ...} => HEADGOAL (
+        resolve_tac ctxt2 [nth IH (i-1)]
+        THEN_ALL_NEW (
+          ((resolve_tac ctxt2 @{thms K_self}) THEN_ALL_NEW (K no_tac))
+          ORELSE'
+          ((
+            (K all_tac)
 
-fun eq_tac' ctxt =
-  TRY o REPEAT_ALL_NEW (resolve_tac ctxt @{thms relator_eq_raw relator_mono})
-  THEN_ALL_NEW resolve_tac ctxt @{thms is_equality_eq};
-fun tac1' ctx = DETERM o eq_tac' ctx;
-fun transfer_step_tac' ctx = tac0 ctx THEN_ALL_NEW tac1' ctx;
+            THEN' resolve_tac ctxt2 @{thms rel_funI}
+            
+            THEN' eresolve_tac ctxt2 @{thms rel_prod.induct}
+
+            THEN' (K (unfold_tac ctxt2 @{thms K_def eq_onp_def}))
+THEN' (K debug_tac)
+            THEN' (clarify_tac ctxt2)
+
+            THEN' (solve_tac ctxt2 prems)
+
+          ) THEN_ALL_NEW (K no_tac))
+ORELSE' (K all_tac)
+        )
+      )) ctxt1 i)
+    )) @{context})
+  \<close>)
+term 0 *)
+  ML_val \<open>Goal.init; print_tac;
+op oo;
+op THEN_ALL_NEW;
+TRY;
+solve_tac;
+unfold_tac;
+clarify_tac;
+Proof_Context.fact_tac;
+clarsimp_tac;
+SUBGOAL;
+Subgoal.subgoal_cmd;
+full_simp_tac;
+op addsimps;
+clear_simpset;
+rewrite_goals_tac;
+simp_tac;
+\<close>
+ML_prf \<open>
+fun tac0 ctxt prems = (
+        K all_tac
+THEN' (K debug_tac)
+        THEN' (resolve_tac ctxt @{thms rel_funI}
+
+        THEN' eresolve_tac ctxt @{thms rel_prod.induct}
+        THEN' (K (unfold_tac ctxt @{thms K_def eq_onp_def}))
+        THEN' clarify_tac ctxt
+
+        THEN' Proof_Context.fact_tac ctxt prems) ORELSE' (resolve_tac ctxt @{thms K_self}));
+SIMPLE_METHOD;
+TRY;
+SOLVE;
+resolve_tac;
+assume_tac;
 \<close>
 
-lemma K_self: "K x x x"  
-  unfolding eq_onp_def by auto
+  ML_prf \<open>
+fun pretty_cterm ctxt ctrm =
+Syntax.pretty_term ctxt (Thm.term_of ctrm)
 
-lemma K_fun:
-  fixes R f g x
-  assumes "R (f x) (g x)"
-  shows "(K x ===> R) f g"
-  using assms unfolding eq_onp_def by auto
+fun pretty_terms ctxt trms =
+Pretty.block (Pretty.commas (map (Syntax.pretty_term ctxt) trms));
 
-term 0 (**)
-lemma "bf.consistentDP bf\<^sub>T"
-  apply (rule bf.consistentDP_intro)
-  subgoal for param
-    apply (rule bf_inductS')
-     apply (unfold bf\<^sub>T.simps)
-    subgoal
-      apply (rule bf.crel_vs_checkmem)
-      apply (unfold bf.simps)
-      apply transfer_prover
-      done
+fun pretty_thm_no_vars ctxt thm =
+let
+val ctxt' = Config.put show_question_marks false ctxt
+in
+Syntax.pretty_term ctxt' (Thm.prop_of thm)
+end
+
+fun pretty_thms_no_vars ctxt thms =
+  Pretty.block (Pretty.commas (map (pretty_thm_no_vars ctxt) thms));
+
+fun pretty_cterms ctxt ctrms =
+  Pretty.block (Pretty.commas (map (pretty_cterm ctxt) ctrms));
+
+fun foc_tac focus =
+    let
+      val {prems, params, asms, concl, context, schematics}: Subgoal.focus = focus;
+      fun assgn1 f1 f2 xs =
+        let
+        val out = map (fn (x, y) => Pretty.enum ":=" "" "" [f1 x, f2 y]) xs
+        in
+        Pretty.list "" "" out
+        end
+
+      fun assgn2 f xs = assgn1 f f xs
+
+      val pps = map (fn (s, pp) => Pretty.block [Pretty.str s, pp])
+        [("params: ", assgn1 Pretty.str (pretty_cterm context) params),
+        ("assumptions: ", pretty_cterms context asms),
+        ("conclusion: ", pretty_cterm context concl),
+        ("premises: ", pretty_thms_no_vars context prems),
+        ("schematics: ", Pretty.str (@{make_string} schematics))
+        ]
+    in
+      tracing (Pretty.string_of (Pretty.chunks pps)); all_tac
+    end
+\<close>
+(*    apply(tactic {* Subgoal.FOCUS foc_tac @{context} 1 *})*)
+  ML_prf \<open>
+val tactac =       resolve_tac @{context} @{thms K_self}
+      ORELSE' (resolve_tac @{context} @{thms rel_funI}
+        THEN' eresolve_tac @{context} @{thms rel_prod.induct}
+        THEN' (SELECT_GOAL (unfold_tac @{context} @{thms K_def eq_onp_def}))
+        THEN' clarsimp_tac @{context})
+;
+\<close>
+    
+  apply (tactic \<open>HEADGOAL (
+    resolve_tac @{context} @{thms bf\<^sub>T.induct}
+    THEN_ALL_NEW (fn i => Subgoal.FOCUS (fn {context=ctx, prems=IH, ...} =>
+      HEADGOAL (resolve_tac ctx [nth IH (i-1)])) @{context} i)
+    THEN_ALL_NEW tactac)\<close>
+)
+supply [[show_types]]
+  apply (tactic \<open>ALLGOALS tactac\<close>)
+  
+  term 0 (*
+  apply (tactic \<open>HEADGOAL (
+    resolve_tac @{context} @{thms bf\<^sub>T.induct}
+    THEN_ALL_NEW (fn i => Subgoal.FOCUS (fn {context=ctx, prems=IH, ...} =>
+      HEADGOAL (resolve_tac ctx [nth IH (i-1)])) @{context} i)
+THEN_ALL_NEW tactac)\<close>)
+      term 0 (*
+    THEN_ALL_NEW (
+      resolve_tac @{context} @{thms K_self}
+      ORELSE' (resolve_tac @{context} @{thms rel_funI}
+        THEN' eresolve_tac @{context} @{thms rel_prod.induct}
+        THEN' (K (unfold_tac @{context} @{thms K_def eq_onp_def}))
+        THEN' clarsimp_tac @{context}
+      )
+      ORELSE' (K (print_tac @{context} "wtf"))
+    )
+)
+\<close>)
+    term 0 (*
+  apply (tactic \<open>Subgoal.FOCUS (fn {context=ctx, prems=IH, ...} =>
+    resolve_tac ctx IH 1) @{context} 1\<close>)
+   apply (tactic \<open>resolve_tac @{context} @{thms K_self} 1\<close>)
+    apply (tactic \<open>Subgoal.FOCUS (fn {context=ctx, prems=IH, ...} =>
+    resolve_tac ctx IH 1) @{context} 1\<close>)
+     apply (tactic \<open>resolve_tac @{context} @{thms K_self} 1\<close>)
+    apply (tactic \<open>resolve_tac @{context} @{thms K_self} 1\<close>)
+    apply (tactic \<open>(resolve_tac @{context} @{thms rel_funI}
+
+        THEN' eresolve_tac @{context} @{thms rel_prod.induct}
+        THEN' (K (unfold_tac @{context} @{thms K_def eq_onp_def}))
+        THEN' clarsimp_tac @{context}
+
+) 1\<close>)+
+      
+term 0 (*
+  apply(tactic \<open>
+    HEADGOAL (Subgoal.FOCUS (fn {context=ctxt, prems=IH, ...} => HEADGOAL (
+      let
+        val _ = @{print} IH;
+      in
+        resolve_tac ctxt @{thms bf\<^sub>T.induct}
+        THEN_ALL_NEW (fn i =>
+          let
+            val _ = @{print} i;
+          in
+            Subgoal.FOCUS (fn {context=ctxt, params, prems, schematics, ...} => HEADGOAL (
+              let
+                val _ = @{print} ("prems", prems, "params", params, "schematics", schematics)
+              in
+                resolve_tac ctxt [nth IH (i-1)]
+                THEN_ALL_NEW (fn i =>
+                  let
+                    val _ = @{print} ("inner", i)
+                  in
+                    Subgoal.FOCUS (fn {context=ctxt, ...} => HEADGOAL (
+                      resolve_tac ctxt @{thms K_self}
+                    )) ctxt i
+                    ORELSE
+                    Subgoal.FOCUS (fn {context=ctxt, ...} =>
+                      HEADGOAL (resolve_tac ctxt @{thms rel_funI})
+                      THEN HEADGOAL (eresolve_tac ctxt @{thms rel_prod.induct})
+                      THEN (unfold_tac ctxt @{thms K_def eq_onp_def})
+                      THEN HEADGOAL (clarify_tac ctxt)
+THEN print_tac ctxt "blah"
+                    ) ctxt i
+                    ORELSE (debug_tac)
+                  end)
+              end
+            )) ctxt i
+          end
+        )
+      end
+    )) @{context})
+\<close>)
+term 0 *)
+*)
+  subgoal premises IH
+    apply (rule bf\<^sub>T.induct)
     subgoal premises prems
-      apply (rule bf.crel_vs_checkmem)
-      apply (unfold bf.simps)
-      supply [transfer_rule] = prems K_self K_fun
-      apply transfer_prover_start
-                          apply transfer_step
-                          apply transfer_step
-                          apply transfer_step back back back back back back back back
-                          apply transfer_step
-                          apply transfer_step
-                          apply transfer_step
-                          apply transfer_step
-                         apply transfer_step back back back back
-                        apply transfer_step
-                       apply transfer_step back back back back back back back back back back back back
-                      apply transfer_step back
-                     apply transfer_step
-                    apply (tactic \<open>HEADGOAL (transfer_step_tac' @{context})\<close>) 
-                   apply transfer_step
-                  apply transfer_step back
-                 apply transfer_step
-                apply transfer_step
-               apply transfer_step
-              supply [transfer_rule] = bf.map_transfer_inset0
-              apply transfer_step
-             apply transfer_step
-            apply transfer_step
-           apply transfer_step back
-          supply [transfer_rule] = bf.fold_transfer
-          apply transfer_step
-         apply transfer_step
-        apply transfer_step
-       apply transfer_step
-      apply transfer_prover_end
+      apply (rule IH(1))
+      subgoal by (rule K_self)
+      done
+      term 0 (**)
+    subgoal premises prems
+      apply (rule IH(2))
+      subgoal by (rule K_self)
+      subgoal by (rule K_self)
+      subgoal
+        apply (rule rel_funI)
+        apply (erule rel_prod.induct)
+        unfolding K_def eq_onp_def
+        apply clarify
+        apply (fact prems)
+        done
+      subgoal
+        apply (rule rel_funI)
+        apply (erule rel_prod.induct)
+        unfolding K_def eq_onp_def
+        apply clarify
+        apply (fact prems)
+        done
       done
     done
   done
+thm eq_onp_to_eq
+  
+interpretation bf: dp_consistency bf .
+lemma "bf.consistentDP bf\<^sub>T"
+  by (dp_match induct: bf_inductS' simp: bf.simps simp\<^sub>T: bf\<^sub>T.simps)
+    
+term 0 (**)
+  thm bf.induct[split_format(complete)] bf.induct
+ML_command \<open>
+val prop = @{thm bf.induct} |> Thm.prop_of;
+val horn = prop |> Logic.strip_horn;
+val horn0 = horn |> fst |> hd;
+val horn00 = horn0 |> Logic.strip_assums_concl;
+@{print} horn0
+\<close>
+ML_command \<open>
+val prop = @{thm bf.consistentDP_intro} |> Thm.prop_of;
+val concl = prop |> Logic.strip_assums_concl;
+val cterm = prop |> Thm.cterm_of @{context};
+cterm |> Goal.init |> Goal.conclude;
+\<close>
+ML_val \<open>
+@{term "True = True"} |> HOLogic.mk_Trueprop |> Thm.cterm_of @{context} |> Goal.init;
+Clasimp.auto_tac;
+op RS;
+@{cterm P};
+resolve_tac;
+Proof.apply;
+\<close>
+ML \<open>
+val pth: tactic = fn th =>
+  let
+    val _ = @{print} th;
+  in
+    all_tac th
+  end
+\<close>
+  
+ML \<open>
+val prop = @{thm bf.induct} |> Thm.prop_of;
+val (IH, thesis) = prop |> Logic.strip_horn;
+val prop' = Logic.list_implies (IH, thesis);
+val cterm' = Thm.cterm_of @{context} prop';
+val tac = HEADGOAL (resolve_tac @{context} @{thms bf.induct});
+fun factac ctxt = Proof_Context.fact_tac ctxt @{thms bf.induct};
+val thm' = Goal.init cterm'
+|> tac |> Seq.hd
+;
+Goal.prove @{context} [] [] prop' (K (HEADGOAL (factac @{context})));
+@{print} it;
+@{print} prop';
+@{print} @{thms bf.induct};
+Variable.variant_frees;
+Term.close_schematic_term prop;
+@{print} it;
+@{print} prop;
+Term.abs;
+Name.is_skolem;
+\<close>
+  
+ML \<open>
+val pp = @{thm bf.induct} |> Thm.prop_of;
+Term.add_vars pp [];
+pp |> Term.close_schematic_term;
+
+fun
+  all_abs (Abs (x, tp, body)) = Logic.all_const tp $ Abs(x, tp, all_abs body)
+| all_abs tm = tm;                          
+
+val ppa = pp |> Term.close_schematic_term |> all_abs;
+val cterm = Thm.cterm_of @{context} ppa;
+
+Goal.prove @{context} [] [] ppa (K (HEADGOAL (factac @{context})));
+\<close>
+  
+ML \<open>
+ppa |> Logic.strip_params;
+ppa |> Logic.strip_assums_hyp;
+ppa |> Logic.strip_assums_concl;
+not true;
+length;
+HOLogic.mk_eq;
+HOLogic.eq_const;
+nth;
+@{const_name K};
+@{const_name Pair};
+Term.type_of;
+HOLogic.boolT;
+@{type_name prod};
+@{term "bf.crel_vs"};
+@{const_name "DP_CRelVS.dp_consistency.crel_vs"};
+op @;
+(Term.strip_type @{typ "'a => 'a => bool"} |> snd) = HOLogic.boolT;
+val s = "s";
+BNF_Util.mk_pred2T;
+op `;
+HOLogic.dest_Trueprop @{prop "None=None"};
+HOLogic.mk_prodT;
+single;
+\<close>
+  
+ML \<open>
+@{method auto};
+Method.check_name;
+Method_Closure.apply_method;
+Proof.apply;
+Method.evaluate;
+Thm.instantiate;
+Rule_Insts.where_rule;
+Term.abs;
+\<close>
+term rel_fun
+thm bf\<^sub>T.induct[of x]
+term 0 (**)
+ML_file \<open>../scratch/Transform_Induct.ML\<close>
+  
+ML_val \<open>
+val prop = transform_induct @{context} @{thm bf\<^sub>T.induct};
+Goal.prove;
+Subgoal.subgoal;
+\<close>    
