DP_Proof.thy
@@ -2,7 +2,6 @@ theory DP_Proof
   imports "./DP_CRelVS" "~~/src/HOL/Eisbach/Eisbach_Tools"
 begin           
 
-term 0 (*
 method dp_match uses induct simp simp\<^sub>T =
   ( rule dp_consistency.consistentDP_intro,
     rule induct,
@@ -11,21 +10,5 @@ method dp_match uses induct simp simp\<^sub>T =
     unfold simp,
     ((match premises in _[transfer_rule]: _ (multi) \<Rightarrow> transfer_prover)
       | (match conclusion in _ \<Rightarrow> transfer_prover)))
-*)
-thm dp_consistency.crel_vs_return
-thm dp_consistency.case_prod_transfer
-thm dp_consistency.crel_vs_fun_app
-term 0 
-method dp_step uses IH =
-  (match conclusion in
-    "dp_consistency.crel_vs dp R x \<langle>y\<rangle>" for dp R x y
-    \<Rightarrow> \<open>rule dp_consistency.crel_vs_return[of R x y dp]\<close>
-  \<bar> "dp_consistency.crel_vs dp R (f x) (f\<^sub>T . x\<^sub>T)" for dp R f x f\<^sub>T x\<^sub>T
-    \<Rightarrow> \<open>match (x) in
-        "f x" \<Rightarrow> fail
-      \<bar> _ \<Rightarrow> \<open>rule dp_consistency.crel_vs_fun_app[where f=f and x=x]\<close>\<close>
-  \<bar> _ \<Rightarrow> \<open>fact dp_consistency.case_prod_transfer\<close>
-  )
 
-method dp_naive = (solves \<open>simp\<close>)
 end
