scratch/Scratch_Tactic_Antiquotation.thy
@@ -1,0 +1,47 @@
+theory Scratch_Tactic_Antiquotation
+  imports Main
+begin
+ML \<open>
+fun pretty_cterm ctxt ctrm =
+Syntax.pretty_term ctxt (Thm.term_of ctrm)
+
+fun pretty_terms ctxt trms =
+Pretty.block (Pretty.commas (map (Syntax.pretty_term ctxt) trms));
+
+fun pretty_thm_no_vars ctxt thm =
+let
+val ctxt' = Config.put show_question_marks false ctxt
+in
+Syntax.pretty_term ctxt' (Thm.prop_of thm)
+end
+
+fun pretty_thms_no_vars ctxt thms =
+  Pretty.block (Pretty.commas (map (pretty_thm_no_vars ctxt) thms));
+
+fun pretty_cterms ctxt ctrms =
+  Pretty.block (Pretty.commas (map (pretty_cterm ctxt) ctrms));
+
+fun foc_tac {prems, params, asms, concl, context, schematics} =
+    let
+      fun assgn1 f1 f2 xs =
+        let
+        val out = map (fn (x, y) => Pretty.enum ":=" "" "" [f1 x, f2 y]) xs
+        in
+        Pretty.list "" "" out
+        end
+
+      fun assgn2 f xs = assgn1 f f xs
+
+      val pps = map (fn (s, pp) => Pretty.block [Pretty.str s, pp])
+        [("params: ", assgn1 Pretty.str (pretty_cterm context) params),
+        ("assumptions: ", pretty_cterms context asms),
+        ("conclusion: ", pretty_cterm context concl),
+        ("premises: ", pretty_thms_no_vars context prems),
+        ("schematics: ", assgn2 (pretty_cterm context) (snd schematics))]
+    in
+      tracing (Pretty.string_of (Pretty.chunks pps)); all_tac
+    end
+\<close>
+  schematic_goal shows "\<And>x y. A x y \<Longrightarrow> B y x \<Longrightarrow> C (?z y) x"
+apply(tactic {* Subgoal.FOCUS foc_tac @{context} 1 *})
+end
