scratch/Scratch_crel_mono.thy
@@ -1,0 +1,16 @@
+theory Scratch_crel_mono
+  imports "../DP_CRelVS"
+begin
+
+context dp_consistency
+begin
+
+lemma crel_vs_mono:
+  fixes R0 R1
+  assumes "R0 \<le> R1"
+  shows "crel_vs R0 \<le> crel_vs R1"
+  using assms by (fastforce intro: crel_vs_intro elim: crel_vs_elim)
+
+end
+
+end
